SndToExe_preserves_INV_4 verifies Code cleanup

opaque.dfy
@@ -10,8 +10,8 @@ abstract module Opaque{
     type Config
     type Actor
     type Frame
-    //old app constructor app(is, b) left in for backwards compatibility
-    //leave only the app(f) in later
+    //old app constructor app(is, b) left in for backwards compatibility 
+    // with earlier versions of the paper
     datatype Msg = orca(i: Addr, z: int) | app(is: set<Addr>, b: BId) | app'(f: Frame)| ERR
     function Heap(c: Config, i: Addr, fid: FId) : Addr
     function allocated_addresses(c: Config) : set<Addr>
@@ -38,58 +38,6 @@ abstract module Opaque{
     //lemma all valid actor addresses are in the domain of Actors
     function Actors(c: Config, a: ActorAddr) : Actor
 
-    //Queues//
-    function queue_length(c: Config, a: ActorAddr) : nat
-    function queue_n(c: Config, a: ActorAddr, n: nat) : Msg
-
-    function prev_message(c: Config, a: ActorAddr, n: nat) : Msg
-    {
-        if n >= 1 then queue_n(c, a, n-1) else Msg.ERR
-    }
-
-    predicate WF_queue(c: Config, a: ActorAddr) {
-        (forall n: nat :: 
-            n < queue_length(c,a) ==> 
-            queue_n(c, a, n) != Msg.ERR) &&
-
-        (forall n: nat :: 
-            n >= queue_length(c,a) ==> 
-            queue_n(c,a,n) == Msg.ERR)
-    }
-
-    predicate push(c: Config, a: ActorAddr, msg: Msg, c': Config)
-    {
-        WF_queue(c, a) &&
-        msg != Msg.ERR &&
-        queue_length(c', a) == queue_length(c, a) + 1 &&
-        queue_n(c', a, queue_length(c,a)) == msg &&
-
-        (forall n: nat :: 
-            n != queue_length(c,a) ==>
-            queue_n(c', a, n) == queue_n(c, a, n))
-    }
-
-    lemma {:verify false} push_preserves_WF_queue(c: Config, a: ActorAddr, msg: Msg, c': Config)
-        requires push(c, a, msg, c')
-        ensures WF_queue(c', a)
-    {
-    }
-
-    predicate pop(c:Config, a:ActorAddr, c': Config)
-    {
-        WF_queue(c, a) &&
-        queue_length(c', a) == queue_length(c, a) - 1 &&
-
-        (forall n: nat ::
-            n >= 0 ==>
-            queue_n(c', a, n) == queue_n(c, a, n+1))
-    }
-
-    lemma {:verify false} pop_preserves_WF_queue(c: Config, a: ActorAddr, c': Config)
-        requires pop(c, a, c')
-        ensures WF_queue(c', a)
-    {
-    }
 
 
     ////REFERENCE COUNTS////
@@ -98,10 +46,20 @@ abstract module Opaque{
     function LRC(c: Config, i: Addr) : int
     function FRC(c: Config, i: Addr) : int
     function AMC(c: Config, i: Addr) : int
-    //{|(set x | exists a,k :: 0<=k<queue_length(c, a) && x==(a,k) && Reach(c,a,k,i))|}
+    
+    lemma LRC_is_owner_RC(c: Config, i: Addr, a: ActorAddr)
+        requires Owner(c, i, a)
+        ensures LRC(c, i) == RC(c, i, a)
+    
+    lemma FRC_is_not_owner_RC(c: Config, i: Addr, actors: set<ActorAddr>) 
+        requires forall a ::    
+                    a in actors <==>
+                    !Owner(c, i, a) 
+        ensures FRC(c, i) == sum_over_set_RC(c, actors)
+    /////////////////////////
 
 
-    ////DATA RACE FREEDOM////
+    /////DATA RACE FREEDOM/////
     predicate DRF(c: Config) {
         forall a, a': ActorAddr, p, p': DP, i: Addr, k: Capability ::
             a != a' &&
@@ -109,10 +67,65 @@ abstract module Opaque{
             A(c, a', p', i, k) ==>
             k == TAG
     }
+    /////////////////////////
+
+
+    //////ACCESSIBILITY////// 
+    predicate A(c: Config, a: ActorAddr, dp: DP, i: Addr, k: Capability)
+
+    predicate accessible_via_lp(c: Config, i: Addr, a: ActorAddr) {
+        exists lp,k ::
+            A(c, a, lp, i, k)
+    }
 
     predicate is_a_message_path(c: Config, mp: DP)
 
+    predicate live(c: Config, a: ActorAddr, i: Addr) {
+        exists k, dp ::
+            A(c, a, dp, i, k)
+    }
+
+    predicate msg_live(c: Config, a: ActorAddr, i: Addr, n: nat) {
+        (exists k, mp ::
+            A(c, a, mp, i, k) &&
+            is_a_message_path(c, mp) &&
+            message_path_from_n(c, mp, n)) ||
+        (queue_at_n_orca(c, a, n) &&
+        queue_at_n_orca_i(c, a, n) == i)
+    }
+
+    predicate message_path_from_n(c: Config, mp: DP, n: nat)
+    /////////////////////////
+
+
     //////////////////////////////INVARIANTS///////////////////////////////
+
+    predicate INV_1() {
+        forall c ::
+            DRF(c)
+    }
+
+    predicate INV_2(c: Config) {
+        forall i, dp, mp, k, a, a_own ::
+            (A(c, a, dp, i, k) &&
+            !Owner(c, i, a)) ||
+            (A(c, a_own, mp, i, k) &&
+            Owner(c, i, a_own) &&
+            is_a_message_path(c, mp)) ==>
+            LRC(c, i) > 0
+    }
+
+    predicate INV_3(c: Config) {
+        forall i, dp, k, a ::
+            A(c, a, dp, i, k) &&
+            !Owner(c, i, a) ==>
+            RC(c, i, a) > 0
+    }
+
+    predicate INV_4(c: Config) {
+        forall i ::
+            LRC(c, i) + OMC(c, i) == FRC(c, i) + AMC(c, i)
+    }
 
     predicate INV_5(c: Config) 
     //RC returns a nat. Therefore, INV_5 holds implicitly
@@ -138,50 +151,8 @@ abstract module Opaque{
                     j <= n ==>
                     LRC_plus_queue_effect(c, a, i, j) > 0)
     }
-
-    ////AUXILIARY FOR INV_6////
-    predicate queue_at_n_orca(c: Config, a: ActorAddr, n: nat)
-        ensures queue_at_n_orca(c, a, n) ==> n <= queue_length(c, a)
-    {
-        WF_queue(c, a) &&
-        queue_n(c, a, n).orca?
-    }
-
-    function queue_at_n_orca_i(c: Config, a: ActorAddr, n: nat) : Addr
-        requires queue_at_n_orca(c, a, n)
-    {
-        queue_n(c, a, n).i
-    }
-
-    function queue_at_n_orca_z(c: Config, a: ActorAddr, n: nat) : int
-        requires queue_at_n_orca(c, a, n)
-    {
-        queue_n(c, a, n).z
-    }
-
-    function queue_effect(c: Config, a: ActorAddr, i: Addr, incl: nat, excl: nat) : int
-
-
-    predicate live(c: Config, a: ActorAddr, i: Addr) {
-        exists k, dp ::
-            A(c, a, dp, i, k)
-    }
-
-    predicate msg_live(c: Config, a: ActorAddr, i: Addr, n: nat) {
-        (exists k, mp ::
-            A(c, a, mp, i, k) &&
-            is_a_message_path(c, mp) &&
-            message_path_from_n(c, mp, n)) ||
-        (queue_at_n_orca(c, a, n) &&
-        queue_at_n_orca_i(c, a, n) == i)
-    }
-
-    predicate message_path_from_n(c: Config, mp: DP, n: nat)
-    //////////////////////////
-    
-    predicate INV_8(c: Config) 
-         
     ///////////////////////////////////////////////////////////////////////////
+
 
     /////SYSTEM PROPERTIES/////
     predicate Ownership_Immutable(c: Config, c': Config)
@@ -196,6 +167,7 @@ abstract module Opaque{
             a != a' ==>
             !Owner(c, i, a')
     ///////////////////////////
+
 
     ///////////////PSEUDO CODE FOR RECEIVING MESSAGES (FIGURE 6)///////////////
 
@@ -236,7 +208,7 @@ abstract module Opaque{
     }
 
 
-    lemma {:verify true} RcvToExe_Increases_A(c: Config, a: ActorAddr, c': Config)
+    lemma RcvToExe_Increases_A(c: Config, a: ActorAddr, c': Config)
         requires RcvToExe(c, a, c')
         ensures forall lp, i, k :: 
             A(c, a, lp, i, k) ==> 
@@ -252,7 +224,7 @@ abstract module Opaque{
             A(c', a', lp, i, k) == A(c, a', lp, i, k)
 
 
-    lemma {:verify false} RcvToExe_Preserves_INV_3(c: Config, a': ActorAddr, c': Config)
+    lemma RcvToExe_Preserves_INV_3(c: Config, a': ActorAddr, c': Config)
         requires INV_3(c)
         requires RcvToExe(c, a', c')
         ensures INV_3(c')
@@ -277,24 +249,6 @@ abstract module Opaque{
     ////AUXILIARY FOR RcvApp////
     predicate actor_state_idle(c: Config, a: ActorAddr)
 
-    predicate queue_at_n_app(c: Config, a: ActorAddr, n: nat)
-        ensures queue_at_n_app(c, a, n) ==> n <= queue_length(c, a)
-    {
-        WF_queue(c, a) &&
-        queue_n(c, a, n).app?
-    }
-
-    function queue_at_n_app_is(c: Config, a: ActorAddr, n: nat) : set<Addr>
-        requires queue_at_n_app(c, a, n)
-    {
-        queue_n(c, a, n).is
-    }
-    
-    function queue_at_n_app_b(c: Config, a: ActorAddr, n: nat) : BId
-        requires queue_at_n_app(c, a, n)
-    {
-        queue_n(c, a, n).b
-    }
 
     predicate actor_state_rcv(c: Config, a: ActorAddr)
 
@@ -338,6 +292,7 @@ abstract module Opaque{
         requires queue_at_n_orca(c, a, 0)
         ensures queue_effect(c, a, queue_at_n_orca_i(c, a, 0), 0, 1) == queue_at_n_orca_z(c, a, 0)
     
+    function queue_effect(c: Config, a: ActorAddr, i: Addr, incl: nat, excl: nat) : int
 
     function LRC_plus_queue_effect(c: Config, a: ActorAddr, i: Addr, excl: nat) : int
     {
@@ -374,10 +329,9 @@ abstract module Opaque{
             i != i' ==>
             (live(c, a, i') <==>
             live(c', a, i'))
-
     //////////////////////////////
 
-    lemma {:verify false} rcvORCA_preserves_INV_6(c: Config, a_own: ActorAddr, c': Config)
+    lemma rcvORCA_preserves_INV_6(c: Config, a_own: ActorAddr, c': Config)
         requires INV_6(c)
         requires INV_2(c)
         requires rcvORCA(c, a_own, c')
@@ -446,98 +400,33 @@ abstract module Opaque{
     ///////////////PSEUDO CODE FOR SENDING MESSAGES (FIGURE 8)///////////////
 
     /////////Auxiliary for ExeToSnd and SndToExe////////// 
-    predicate actor_state_snd(c: Config, a: ActorAddr)
+    //these can be probably generalised into fewer methods - that is for later    
 
-    function actor_state_snd_frame(c: Config, a: ActorAddr) : Frame
-        requires actor_state_snd(c, a)
+    predicate actor_state_snd(c: Config, a: ActorAddr)
 
     function actor_state_snd_msg(c: Config, a: ActorAddr) : Msg 
         requires actor_state_snd(c, a)
-
-    function actor_state_snd_msg_b(c: Config, a: ActorAddr) : BId
-        requires actor_state_snd(c, a)
-
-    function actor_state_snd_msg_is(c: Config, a: ActorAddr) : set<Addr>
-        requires actor_state_snd(c, a)
-
-    //function actor_ws(c: Config, a: ActorAddr) : set<Addr>
-    //    requires actor_state_snd(c, a)
 
     function actor_state_snd_f'(c: Config, a: ActorAddr) : Frame
         requires actor_state_snd(c, a)
 
     function actor_state_snd_a'(c: Config, a: ActorAddr) : ActorAddr
         requires actor_state_snd(c, a)
-
-    predicate msg_live_app(c: Config, a: ActorAddr, i: Addr, n: nat) {
-        msg_live(c, a, i, n) &&
-        queue_n(c, a, n).app?
-    }
-    
-    predicate A(c: Config, a: ActorAddr, dp: DP, i: Addr, k: Capability)
-
-    predicate accessible_via_lp(c: Config, i: Addr, a: ActorAddr) {
-        exists lp,k ::
-            A(c, a, lp, i, k)
-    }
-    
-    predicate split(f: Frame, f': Frame, f'': Frame) 
-    predicate ExeToSnd'(c: Config, a: ActorAddr, a': ActorAddr, c': Config, c'': Config) 
-        requires actor_state_exe(c, a)
-        requires queue_at_n_app(c'', a', queue_length(c, a'))
-        requires forall x ::
-                    x in queue_at_n_app_f_rng(c'', a', queue_length(c, a')) ==>
-                    x in actor_state_exe_f_rng(c, a)
-        requires forall x ::
-                    x in queue_at_n_app_f_dom(c'', a', queue_length(c, a')) ==>
-                    x !in actor_state_exe_f_dom(c, a)
-
-    predicate subset(Set: set<Addr>, subset: set<Addr>) {
-        forall iota ::  
-            iota in subset ==>
-            iota in Set
-    }
-
-    predicate disjoint(Set: set<Addr>, Set': set<Addr>) {
-        forall iota ::  
-            iota in Set ==>
-            iota !in Set'
-    }
-    
-    function union(Set: set<Addr>, Set': set<Addr>) : set<Addr>
-    ensures forall iota ::
-            (iota in Set || 
-            iota in Set') ==>
-            iota in union(Set, Set')
-
-//these can be probably generalised into fewer methods - that is for later    
-    function msg_frame_rng(c: Config, msg: Msg) : set<Addr>
-    function msg_frame_dom(c: Config, msg: Msg) : set<Addr>
+     
+    function msg_f(c: Config, msg: Msg) : Frame
 
     function actor_state_snd_f(c: Config, a: ActorAddr) : Frame 
-    
-    function actor_state_snd_f_rng(c: Config, a: ActorAddr) : set<Addr>
-        requires actor_state_snd(c, a)
-
-    function actor_state_snd_f_dom(c: Config, a: ActorAddr) : set<Addr>
-        requires actor_state_snd(c, a)
 
     function actor_state_exe_f(c: Config, a: ActorAddr) : Frame 
 
-    function actor_state_exe_f_rng(c: Config, a: ActorAddr) : set<Addr>
-        requires actor_state_exe(c, a)
-
-    function actor_state_exe_f_dom(c: Config, a: ActorAddr) : set<Addr>
-        requires actor_state_exe(c, a)
-
-    function queue_at_n_app_f_rng(c: Config, a: ActorAddr, n: nat) : set<Addr>
-        requires queue_at_n_app(c, a, n)
-
-    function queue_at_n_app_f_dom(c: Config, a: ActorAddr, n: nat) : set<Addr>
-        requires queue_at_n_app(c, a, n)
-    
     function queue_at_n_app_f(c: Config, a: ActorAddr, n: nat) : Frame
         requires queue_at_n_app(c, a, n)
+
+    function frame_dom(f: Frame) : set<VarId>
+
+    function frame_rng(f: Frame) : set<Addr>
+
+    ////////////////////////////////////////////////////// 
 
     ////ExeToSnd////
     predicate ExeToSnd(c: Config, a: ActorAddr, a': ActorAddr, c': Config, c'': Config, msg: Msg) 
@@ -545,8 +434,8 @@ abstract module Opaque{
         requires queue_at_n_app(c'', a', queue_length(c, a'))
         requires push(c, a', msg, c'') 
         requires msg.app?
-        requires subset(msg_frame_rng(c, msg), actor_state_exe_f_rng(c, a))
-        requires disjoint(msg_frame_dom(c, msg), actor_state_exe_f_dom(c, a))
+        requires subset(frame_rng(msg_f(c, msg)), frame_rng(actor_state_exe_f(c, a)))
+        requires disjoint(frame_dom(msg_f(c, msg)), frame_dom(actor_state_exe_f(c, a)))
         requires DRF(c'')
         
     {
@@ -559,11 +448,10 @@ abstract module Opaque{
     }
 
     ////SndToExe////
-    predicate SndToExe(c: Config, a: ActorAddr, a': ActorAddr, c': Config, c'': Config, msg: Msg) 
+    predicate SndToExe(c: Config, a: ActorAddr, a': ActorAddr, c': Config, c'': Config) 
     {
         actor_state_snd(c, a) &&
         actor_state_snd_a'(c, a) == a' &&
-        actor_state_snd_msg(c, a) == msg &&
 
         all_else_unmodified(c, a, c') &&
         Ownership_Immutable(c, c') &&
@@ -572,40 +460,75 @@ abstract module Opaque{
         var f' := actor_state_snd_f'(c, a);
         var ws := actor_ws(c, a);
         
-                
-        msg.app'? &&
-        msg.f == f' &&
-        
         (forall i :: 
             i in ws && 
             Owner(c, i, a) ==> 
-            RC(c', i, a) == RC(c, i, a) + 1) &&
+            RC(c', i, a) == RC(c, i, a) + 1 &&
+            FRC(c', i) == FRC(c, i) &&
+            OMC(c', i) == OMC(c, i) &&
+            LRC(c', i) == LRC(c, i) + 1) &&
 
         (forall i :: 
             i in ws &&
             !Owner(c, i, a) &&
             RC(c, i, a) > 1 ==>
-            RC(c', i, a) == RC(c, i, a) - 1) &&
+            RC(c', i, a) == RC(c, i, a) - 1 &&
+            OMC(c', i) == OMC(c, i) &&
+            LRC(c', i) == LRC(c, i) &&
+            FRC(c', i) == FRC(c, i) - 1) &&
     
-        (forall i, a_own :: 
+        (forall i :: 
             i in ws &&
-            Owner(c, i, a_own) &&
-            a != a_own &&
-            RC(c, i, a) <= 1 ==>
-            RC(c', i, a) == RC(c, i, a) + 256 &&
-            push(c, a_own, orca(i, 256), c')) &&
+            !Owner(c, i, a) &&
+            RC(c, i, a) == 1 ==>
+            RC(c', i, a) == RC(c, i, a) + 255 &&
+            OMC(c', i) == OMC(c, i) + 256 &&
+            LRC(c', i) == LRC(c, i) &&
+            FRC(c', i) == FRC(c, i) + 255) &&
 
         actor_state_exe_f(c', a) == f &&
-        push(c, a', msg, c')
+
+        (forall i ::
+            i in ws ==>
+            AMC(c', i) == AMC(c, i) + 1)
     }
 
+    lemma SndToExe_preserves_INV_4(c: Config, a: ActorAddr, a': ActorAddr, c': Config, c'': Config, f': Frame)
+        requires INV_4(c)
+        requires SndToExe(c, a, a', c', c'')
+        requires ws_WF(c, a, actor_state_snd_f(c, a), actor_state_snd_f'(c, a))
+        ensures INV_4(c') 
+    {
+        forall i |
+        true 
+        ensures LRC(c', i) + OMC(c', i) == FRC(c', i) + AMC(c', i) 
+        {   
+            if (i in actor_ws(c, a)) {
+                if(Owner(c, i, a)) {
+                } else {
+                    if RC(c, i, a) > 1 {
+                    } else {
+                        can_reach_ws(c);
+                    }
+                }
+            } else {
+            }
+        }
+    }
+
+    lemma can_reach_ws(c: Config) 
+        ensures forall a ::
+                (actor_state_snd(c, a) ||
+                actor_state_rcv(c, a)) ==>
+                forall i ::
+                    i in actor_ws(c, a) ==>
+                    RC(c, i, a) >= 1
+        
 
     predicate Reachable(c: Config, iota: Addr, a: ActorAddr, f: Frame)
 
-    function frame_union_domain(c: Config, f: Frame, f': Frame) : set<Addr>
     function all_reachable(c: Config, a: ActorAddr, f: Frame) : set<Addr>
-    function frame_dom(f: Frame) : set<VarId>
-    function frame_rng(f: Frame) : set<Addr>
+
 
     predicate ws_WF(c: Config, a: ActorAddr, f: Frame, f': Frame)
         requires actor_state_snd(c, a)
@@ -638,72 +561,9 @@ abstract module Opaque{
                 iota in actor_ws(c, a) <==>
                 Reachable(c, iota, a, msg.f)
 
-    //IF I PUSHED CHANGED RC FORALL REACHABLE - USE THIS 
-    lemma SndToExe_preserves_INV_4(c: Config, a: ActorAddr, a': ActorAddr, c': Config, c'': Config, f': Frame, msg: Msg)
-        requires INV_4(c)
-        requires SndToExe(c, a, a', c', c'', msg)
-        requires ws_WF(c, a, actor_state_snd_f(c, a), actor_state_snd_f'(c, a))
-        ensures INV_4(c') 
-    {
-        forall i |
-        true 
-        ensures LRC(c', i) + OMC(c', i) == FRC(c', i) + AMC(c', i) 
-        {
-            if (i in actor_ws(c, a)) {
-                if (!Owner(c, i, a)) {
-                    if (RC(c, i, a) > 1) {
-                        assume false;
-                    } else if RC(c, i, a) <= 1 {
-                        assume false;
-                    }
-                } else {
-                    assert msg.app'?;
-                    assert push(c, a', msg, c');
-                    push_app_inc_AMC(c, a, a', msg, c');
-                    LRC_is_owner_RC(c, i, a);
-                    LRC_is_owner_RC(c', i, a);
-                    assert LRC(c', i) == LRC(c, i) + 1; 
-                    ws_is_reachable_from_msg(c, a, msg);
-                    assert i in actor_ws(c, a); 
-                    assert Reachable(c, i, a, msg.f);
-                    assert AMC(c', i) == AMC(c, i) + 1;
-
-                    assert LRC(c, i) + OMC(c, i) + 1 == LRC(c', i) + OMC(c', i);
-                    assert FRC(c, i) + AMC(c, i) + 1 == FRC(c', i) + AMC(c', i);
-                }            
-            } else {
-            }
-        }
-    }
-
-    function config_actors(c: Config) : set<ActorAddr>
-    function config_actors_excluding(c: Config, a: ActorAddr) : set<ActorAddr>
-        ensures forall a' ::
-                a' in config_actors_excluding(c, a) ==>
-                a != a'
-
-    lemma FRC_is_not_owner_RC(c: Config, i: Addr, actors: set<ActorAddr>) 
-        requires forall a ::    
-                    a in actors <==>
-                    !Owner(c, i, a) 
-        ensures FRC(c, i) == sum_over_set_RC(c, actors)
 
     function sum_over_set_RC(c: Config, actors: set<ActorAddr>) : nat
     
-    lemma sum_over_unmodified_set_unmodified(c: Config, c': Config, actors: set<ActorAddr>)
-        requires forall a ::
-                    a in actors ==>
-                    unchanged_actor(c, a, c')
-        ensures sum_over_set_RC(c, actors) == sum_over_set_RC(c', actors)
-
-    lemma LRC_is_owner_RC(c: Config, i: Addr, a: ActorAddr)
-        requires Owner(c, i, a)
-        ensures LRC(c, i) == RC(c, i, a)
-  
-    //?? when will the set of actors in config be changed?
-    lemma config_actors_unchanged(c: Config, c': Config)    
-            ensures config_actors(c) == config_actors(c') 
-
     predicate all_else_unmodified(c: Config, modified: ActorAddr, c': Config) 
     {
         (forall a ::
@@ -754,96 +614,127 @@ abstract module Opaque{
             a' != a ==> 
             RC(c', i, a') == RC(c, i, a'))
     }
+
+
+    ////////////////////ABSTRACT ADTs/////////////////////
+
+    ///////////SETS///////////
+    predicate subset(Set: set<Addr>, subset: set<Addr>) {
+        forall iota ::  
+            iota in subset ==>
+            iota in Set
+    }
+
+    predicate disjoint(Set: set<VarId>, Set': set<VarId>) {
+        forall iota ::  
+            iota in Set ==>
+            iota !in Set'
+    }
     
-    predicate INV_2(c: Config) {
-        forall i, dp, mp, k, a, a_own ::
-            (A(c, a, dp, i, k) &&
-            !Owner(c, i, a)) ||
-            (A(c, a_own, mp, i, k) &&
-            Owner(c, i, a_own) &&
-            is_a_message_path(c, mp)) ==>
-            LRC(c, i) > 0
+    function union(Set: set<Addr>, Set': set<Addr>) : set<Addr>
+    ensures forall iota ::
+            (iota in Set || 
+            iota in Set') ==>
+            iota in union(Set, Set')
+    /////////////////////////
+
+    /////////QUEUES/////////
+    function queue_length(c: Config, a: ActorAddr) : nat
+
+    //nth message in the queue
+    function queue_n(c: Config, a: ActorAddr, n: nat) : Msg
+
+    function prev_message(c: Config, a: ActorAddr, n: nat) : Msg
+    {
+        if n >= 1 then queue_n(c, a, n-1) else Msg.ERR
     }
 
-    predicate INV_3(c: Config) {
-        forall i, dp, k, a ::
-            A(c, a, dp, i, k) &&
-            !Owner(c, i, a) ==>
-            RC(c, i, a) > 0
+    predicate WF_queue(c: Config, a: ActorAddr) {
+        (forall n: nat :: 
+            n < queue_length(c,a) ==> 
+            queue_n(c, a, n) != Msg.ERR) &&
+
+        (forall n: nat :: 
+            n >= queue_length(c,a) ==> 
+            queue_n(c,a,n) == Msg.ERR)
+    }
+
+    predicate push(c: Config, a: ActorAddr, msg: Msg, c': Config)
+    {
+        WF_queue(c, a) &&
+        msg != Msg.ERR &&
+        queue_length(c', a) == queue_length(c, a) + 1 &&
+        queue_n(c', a, queue_length(c,a)) == msg &&
+
+        (forall n: nat :: 
+            n != queue_length(c,a) ==>
+            queue_n(c', a, n) == queue_n(c, a, n))
+    }
+
+    lemma {:verify false} push_preserves_WF_queue(c: Config, a: ActorAddr, msg: Msg, c': Config)
+        requires push(c, a, msg, c')
+        ensures WF_queue(c', a)
+    {
+    }
+
+    predicate pop(c:Config, a:ActorAddr, c': Config)
+    {
+        WF_queue(c, a) &&
+        queue_length(c', a) == queue_length(c, a) - 1 &&
+
+        (forall n: nat ::
+            n >= 0 ==>
+            queue_n(c', a, n) == queue_n(c, a, n+1))
+    }
+
+    lemma {:verify false} pop_preserves_WF_queue(c: Config, a: ActorAddr, c': Config)
+        requires pop(c, a, c')
+        ensures WF_queue(c', a)
+    {
+    }
+
+    predicate queue_at_n_orca(c: Config, a: ActorAddr, n: nat)
+        ensures queue_at_n_orca(c, a, n) ==> n <= queue_length(c, a)
+    {
+        WF_queue(c, a) &&
+        queue_n(c, a, n).orca?
+    }
+
+    function queue_at_n_orca_i(c: Config, a: ActorAddr, n: nat) : Addr
+        requires queue_at_n_orca(c, a, n)
+    {
+        queue_n(c, a, n).i
+    }
+
+    function queue_at_n_orca_z(c: Config, a: ActorAddr, n: nat) : int
+        requires queue_at_n_orca(c, a, n)
+    {
+        queue_n(c, a, n).z
     }
 
 
-    predicate INV_4(c: Config) {
-        forall i ::
-            LRC(c, i) + OMC(c, i) == FRC(c, i) + AMC(c, i)
+    predicate queue_at_n_app(c: Config, a: ActorAddr, n: nat)
+        ensures queue_at_n_app(c, a, n) ==> n <= queue_length(c, a)
+    {
+        WF_queue(c, a) &&
+        queue_n(c, a, n).app?
     }
+
+    function queue_at_n_app_is(c: Config, a: ActorAddr, n: nat) : set<Addr>
+        requires queue_at_n_app(c, a, n)
+    {
+        queue_n(c, a, n).is
+    }
+    
+    function queue_at_n_app_b(c: Config, a: ActorAddr, n: nat) : BId
+        requires queue_at_n_app(c, a, n)
+    {
+        queue_n(c, a, n).b
+    }
+    /////////////////////////
+
+    ////////////////////////////////////////////////////// 
 
 }
 
 
- /*   
-    ////ExeToSnd////
-    predicate ExeToSnd(c: Config, a: ActorAddr, a': ActorAddr, c': Config, c'': Config) 
-        requires actor_state_exe(c, a)
-        requires queue_at_n_app(c'', a', queue_length(c, a'))
-        requires forall i :: 
-                    i in queue_at_n_app_is(c'', a', queue_length(c, a')) ==>
-                    accessible_via_lp(c'', i, a)
-
-        requires DRF(c'')
-    {
-        actor_state_snd(c', a) &&
-
-        (forall i ::
-                i in actor_ws(c', a) ==>
-                accessible_via_lp_deep(c, i, a)) &&
-        
-        (forall i :: 
-                i in actor_state_snd_msg_is(c', a) ==>
-                accessible_via_lp(c, i, a)) &&
-
-        actor_state_snd_frame(c', a) == actor_state_exe_f(c, a) 
-        
-    }
-
-    
-    ////SndToExe////
-    predicate SndToExe(c: Config, a: ActorAddr, a': ActorAddr, c': Config) {
-        actor_state_snd(c, a) &&
-        Ownership_Immutable(c, c') &&
-        state_atomic(c, a, c') &&
-
-        (forall i :: 
-            i in actor_ws(c, a) && 
-            Owner(c, i, a) ==> 
-            RC(c', i, a) == RC(c, i, a) + 1) &&
-
-        (forall i :: 
-            i in actor_ws(c, a) &&
-            !Owner(c, i, a) &&
-            RC(c, i, a) > 1 ==>
-            RC(c', i, a) == RC(c, i, a) - 1) &&
-    
-        (forall i, a_own :: 
-            i in actor_ws(c, a) &&
-            Owner(c, i, a_own) &&
-            !Owner(c, i, a) &&
-            RC(c, i, a) <= 1 ==>
-
-            RC(c', i, a) == RC(c, i, a) + 256 &&
-
-            queue_at_n_orca(c', a, 0) &&
-            queue_at_n_orca_i(c', a, 0) == i &&
-            queue_at_n_orca_z(c', a, 0) == 256) &&
-            
-            var a' := actor_state_snd_a'(c, a); 
-            var l := queue_length(c, a');
-
-            queue_at_n_app(c', a', l) &&
-            queue_at_n_app_is(c', a', l) == actor_state_snd_msg_is(c, a) &&
-            queue_at_n_app_b(c', a', l) == actor_state_snd_msg_b(c, a) &&
-
-            actor_state_exe(c', a) 
-            //actor_state_exe_f(c', a) == actor_state_snd_frame(c, a)
-    }
-*/
